Impl/BucketIteratorImpl.i.dfy
@@ -1,0 +1,198 @@
+// Copyright 2018-2021 VMware, Inc., Microsoft Inc., Carnegie Mellon University, ETH Zurich, and University of Washington
+// SPDX-License-Identifier: BSD-2-Clause
+
+include "BucketIteratorModel.i.dfy"
+include "../lib/Buckets/TranslationImpl.i.dfy"
+
+module BucketIteratorImpl {
+  import BucketIteratorModel
+  import opened Options
+  import opened Sequences
+  import opened NativeTypes
+  import opened KeyType
+  import opened BucketsLib
+  import opened BucketImpl
+  import opened TranslationLib
+  import opened TranslationImpl
+
+  datatype Iterator = Iterator(
+    pset: Option<PrefixSet>,
+    ghost next: BucketIteratorModel.IteratorOutput,
+    i: uint64,
+    ghost decreaser: int)
+
+  function IIterator(it: Iterator) : BucketIteratorModel.Iterator
+  {
+    BucketIteratorModel.Iterator(it.pset, it.next, it.i as int, it.decreaser)
+  }
+
+  linear datatype BucketIter = BucketIter(it: Iterator, pkv: PackedKV.Pkv, ghost bucket: Bucket)
+  {
+    predicate WFIter()
+    {
+      && PackedKV.WF(pkv)
+      && bucket == PackedKV.I(pkv)
+      && BucketIteratorModel.WFIter(bucket, IIterator(it))
+    } 
+
+    linear method Free()
+    {
+      linear var BucketIter(_,_,_) := this;
+    }
+
+    static function method makeIter(ghost bucket: Bucket, pset: Option<PrefixSet>, idx: uint64): (it': Iterator)
+    requires WFBucket(bucket)
+    requires |bucket.keys| == |bucket.msgs|
+    requires 0 <= idx as int <= |bucket.keys|
+    requires idx as int < |bucket.keys| && pset.Some? 
+        ==> IsPrefix(pset.value.prefix, bucket.keys[idx])
+    ensures IIterator(it')
+      == BucketIteratorModel.iterForIndex(bucket, pset, idx as int)
+    {
+      Iterator(
+          pset,
+          (if idx as int == |bucket.keys| then BucketIteratorModel.Done
+              else BucketIteratorModel.Next(ApplyPrefixSet(pset, bucket.keys[idx]), bucket.msgs[idx])),
+          idx,
+          |bucket.keys| - idx as int)
+    }
+
+    static method IterNextWithPrefix(ghost bucket: Bucket, pkv: PackedKV.Pkv, prefix: Key, idx: uint64) returns (i: uint64)
+    requires WFBucket(bucket)
+    requires PackedKV.WF(pkv)
+    requires PackedKV.I(pkv) == bucket
+    requires 0 <= idx as int <= |bucket.keys|
+    ensures idx as int <= i as int <= |bucket.keys|
+    ensures i as int == BucketIteratorModel.iterNextWithPrefix(bucket, prefix, idx as int)
+    {
+      var len := PackedKV.NumKVPairs(pkv);
+      if idx < len {
+        var key : Key := PackedKV.GetKey(pkv, idx);
+        var isprefix := |prefix| as uint64 <= |key| as uint64 && prefix == key[..|prefix|];
+        reveal_IsPrefix();
+
+        if isprefix {
+          return idx;
+        } 
+
+        var c := PackedKV.KeyspaceImpl.cmp(key, prefix);
+        if c < 0 {
+          var i := PackedKV.PSA.BinarySearchIndexOfFirstKeyGteWithLowerBound(pkv.keys, prefix, idx+1);
+          if i < len {
+            key := PackedKV.GetKey(pkv, i);
+            isprefix := |prefix| as uint64 <= |key| as uint64 && prefix == key[..|prefix|];
+            if isprefix {
+              return i;
+            }
+          }
+        }
+      }
+      return len;
+    }
+
+    static method IterStart(shared bucket: MutBucket, pset: Option<PrefixSet>) returns (linear biter: BucketIter)
+    requires bucket.Inv()
+    ensures biter.WFIter()
+    ensures biter.bucket == bucket.I()
+    ensures IIterator(biter.it) == BucketIteratorModel.IterStart(biter.bucket, pset)
+    {
+      BucketIteratorModel.reveal_IterStart();
+
+      ghost var b := bucket.I();
+      var pkv := bucket.GetPkv();
+
+      var i;
+      if pset.None? {
+        i := 0;
+      } else {
+        i := IterNextWithPrefix(bucket.bucket, pkv, pset.value.prefix, 0);
+      }
+
+      var it := makeIter(b, pset, i);
+      biter := BucketIter(it, pkv, b);
+    }
+
+    static method IterFindFirstGte(shared bucket: MutBucket, pset: Option<PrefixSet>, key': Key)
+    returns (linear biter: BucketIter)
+    requires bucket.Inv()
+    requires pset.Some? ==> IsPrefix(pset.value.prefix, key')
+    ensures biter.WFIter()
+    ensures biter.bucket == bucket.I()
+    ensures IIterator(biter.it) == BucketIteratorModel.IterFindFirstGte(biter.bucket, pset, ApplyPrefixSet(pset, key'))
+    {
+      BucketIteratorModel.reveal_IterFindFirstGte();
+      ghost var b := bucket.I();
+      var pkv := bucket.GetPkv();
+
+      ghost var key := ApplyPrefixSet(pset, key');
+      assert ApplyPrefixSet(RevPrefixSet(pset), key) == key' by { reveal_IsPrefix(); }
+
+      var i: uint64 := PackedKV.PSA.BinarySearchIndexOfFirstKeyGte(pkv.keys, key');  
+      if pset.Some? {
+        i := IterNextWithPrefix(bucket.bucket, pkv, pset.value.prefix, i);
+      }
+
+      var it := makeIter(b, pset, i);
+      biter := BucketIter(it, pkv, b);
+    }
+
+    static method IterFindFirstGt(shared bucket: MutBucket, pset: Option<PrefixSet>, key': Key) returns (linear biter: BucketIter)
+    requires bucket.Inv()
+    requires pset.Some? ==> IsPrefix(pset.value.prefix, key')
+    ensures biter.WFIter()
+    ensures biter.bucket == bucket.I()
+    ensures IIterator(biter.it) == BucketIteratorModel.IterFindFirstGt(biter.bucket, pset, ApplyPrefixSet(pset, key'))
+    {
+      BucketIteratorModel.reveal_IterFindFirstGt();
+      ghost var b := bucket.I();
+      var pkv := bucket.GetPkv();
+
+      ghost var key := ApplyPrefixSet(pset, key');
+      assert ApplyPrefixSet(RevPrefixSet(pset), key) == key' by { reveal_IsPrefix(); }
+
+      var i: uint64 := PackedKV.PSA.BinarySearchIndexOfFirstKeyGt(pkv.keys, key');
+      if pset.Some? {
+        i := IterNextWithPrefix(bucket.bucket, pkv, pset.value.prefix, i);
+      }
+
+      var it := makeIter(b, pset, i);
+      biter := BucketIter(it, pkv, b);
+    }
+
+    linear inout method IterInc()
+    requires old_self.WFIter()
+    requires IIterator(old_self.it).next.Next?
+    ensures self.WFIter()
+    ensures old_self.bucket == self.bucket
+    ensures IIterator(self.it) == BucketIteratorModel.IterInc(old_self.bucket, IIterator(old_self.it))
+    {
+      BucketIteratorModel.lemma_NextFromIndex(self.bucket, IIterator(self.it));
+      BucketIteratorModel.reveal_IterInc();
+
+      var i;
+      if self.it.pset.None? {
+        i := self.it.i + 1;
+      } else {
+        i := IterNextWithPrefix(self.bucket, self.pkv, self.it.pset.value.prefix, self.it.i+1);
+      }
+
+      inout self.it := makeIter(self.bucket, self.it.pset, i);
+    }
+
+    shared method GetNext() returns (next : BucketIteratorModel.IteratorOutput)
+    requires this.WFIter()
+    ensures next == IIterator(this.it).next
+    {
+      BucketIteratorModel.lemma_NextFromIndex(bucket, IIterator(it));
+        
+      if it.i == |pkv.keys.offsets| as uint64 {
+        next := BucketIteratorModel.Done;
+      } else {
+        var key := PackedKV.GetKey(pkv, it.i);
+        var msg := PackedKV.GetMessage(pkv, it.i);
+        next := BucketIteratorModel.Next(ApplyPrefixSet(it.pset, key), msg);
+      }
+    }
+  }
+
+}
